Added new theorems witnessing the fact that the three basic primitive recursive functions are loop computable cleanly.

Loop/Alternative.lean
@@ -104,92 +104,16 @@ def loop_computable (f : Mathlib.Vector Nat n → Nat) : Prop :=
   ∃ p : Program, ⟦ p ⟧^(n) = f
 
 -- -- -------
--- def highest_var : Program → Nat
---   | [] => 0
---   | clear_var k :: tail =>
---     have : lines_of_code tail < lines_of_code (clear_var k :: tail) := by simp
---     max k (highest_var tail)
---   | increment_var k :: tail =>
---     have : lines_of_code tail < lines_of_code (increment_var k :: tail) := by simp
---     max k (highest_var tail)
---   | loop_var k inner :: tail =>
---     have : lines_of_code inner < lines_of_code (loop_var k inner :: tail) := by simp_arith
---     have : lines_of_code tail < lines_of_code (loop_var k inner :: tail) := by simp_arith
---     max k (max (highest_var inner) (highest_var tail))
--- termination_by p => lines_of_code p
-
--- abbrev List.zeros (n : Nat) : List Nat := List.replicate n 0
-
--- -- /- A function is loop computable cleanly if it does not modify the initial state,. -/
--- def loop_computable_cleanly (f : Mathlib.Vector Nat n → Nat) : Prop :=
---   ∃ p : Program, ∀ v : Mathlib.Vector Nat n,
---     execution_from_state (init_state v ++ List.zeros (highest_var p - n)) p
---     =
---     f v :: v.toList ++ List.zeros (highest_var p - n)
-
--- theorem value_at_nil : value_at [] n = 0 := rfl
--- theorem value_at_cons_zero : value_at (x :: xs) 0 = x := rfl
--- theorem value_at_cons_succ : value_at (x :: xs) (n + 1) = value_at xs n := rfl
-
--- theorem value_at_zeros_is_zero (n k : Nat) : value_at (List.zeros n) k = 0 := by
---   revert n
---   induction k
---   case zero =>
---     intro n
---     cases n <;> simp [value_at]
---   case succ ih =>
---     intro n
---     cases n
---     · simp [value_at]
---     · simp [List.replicate, value_at_cons_succ]
---       apply ih
-
--- theorem append_zeros_does_not_change_value_at (xs : VarState) (n k : Nat) :
---     value_at xs k = value_at (xs ++ List.zeros n) k := by
---   revert k
---   induction xs
---   case nil => simp [value_at_nil, value_at_zeros_is_zero]
---   case cons head tail tail_ih =>
---     intro k
---     cases k
---     all_goals simp [value_at_cons_zero, value_at_cons_succ]
---     apply tail_ih
-
-
--- theorem same_values_same_execution (p : Program) (xs ys : VarState) (k : Nat) :
---     (∀ k : Nat, value_at xs k = value_at ys k) → value_at (execution_from_state xs p) k = value_at (execution_from_state ys p) k := by
---   intro ih
---   induction p
---   case nil =>
---     simp [execution_from_state, ih]
---   case cons head tail tail_ih =>
---     cases head
---     all_goals simp [execution_from_state]
---     ·
---       sorry
---     ·
---       sorry
---     ·
---       sorry
-
-
-
--- theorem append_zeros_does_not_change_execution (n k : Nat) :
---     value_at (execution_from_state (xs ++ List.zeros n) p) k = value_at (execution_from_state xs p) k := by
---   have := append_zeros_does_not_change_value_at xs n
---   have := same_values_same_execution p xs (xs ++ List.zeros n) k this
---   exact this.symm
-
--- theorem loop_computable_cleanly_is_loop_computable : loop_computable_cleanly f → loop_computable f := by
---   rename_i n
---   intro ⟨p, h⟩
---   exists p
---   apply funext
---   intro v
---   let dif := highest_var p - n
---   exact
---     calc
---       ⟦ p ⟧^(n) v = value_at (execution_from_state (init_state v) p) 0 := by rw [nary_program_function]
---                 _ = value_at (execution_from_state (init_state v ++ List.zeros dif) p) 0 := by rw [append_zeros_does_not_change_execution ]
---                 _ = value_at (f v :: v.toList ++ List.zeros dif) 0 := by rw [h v]
---                 _ = f v := by rfl
+def highest_var : Program → Nat
+  | [] => 0
+  | clear_var k :: tail =>
+    have : lines_of_code tail < lines_of_code (clear_var k :: tail) := by simp
+    max k (highest_var tail)
+  | increment_var k :: tail =>
+    have : lines_of_code tail < lines_of_code (increment_var k :: tail) := by simp
+    max k (highest_var tail)
+  | loop_var k inner :: tail =>
+    have : lines_of_code inner < lines_of_code (loop_var k inner :: tail) := by simp_arith
+    have : lines_of_code tail < lines_of_code (loop_var k inner :: tail) := by simp_arith
+    max k (max (highest_var inner) (highest_var tail))
+termination_by p => lines_of_code p
